code/ecdsap256/Hacl.Impl.P256.Field.fsti
@@ -39,6 +39,12 @@ val fmod_short: x:felem -> res:felem -> Stack unit
     as_nat h1 res == as_nat h0 x % S.prime)
 
 
+val is_felem_lt_prime_vartime: f:felem -> Stack bool
+  (requires fun h -> live h f)
+  (ensures  fun h0 r h1 -> modifies0 h0 h1 /\
+    r == (as_nat h0 f < S.prime))
+
+
 // NOTE: changed precondition `eq_or_disjoint x y`
 val fadd: x:felem -> y:felem -> res:felem -> Stack unit
   (requires fun h ->
